 \FloatBarrier
\label{sec:2sexlinearother}
Once two-sex linear $r$ has been found for the given $\sigma$, one may
proceed to find the corrsponding both-sex $T$ using:
\todo{maybe remove the sigmas altogether from this equation?}
\begin{equation}
T = \frac{\splitfrac{
   \big((1 - \sigma)  \int _{y'=0}^\infty \int_{a'=y'}^\infty 
       a'e^{-ra'} (1-\varsigma)d_{a'}^F \left( f_{y'}^{F-F} + f_{y'}^{F-M}
       \right) \dd a'\dd y'}{ + \sigma \int_{y=0}^\infty \int _{a=y}^\infty a
       e^{-ra}\varsigma d_{a}^M \left( f_{y}^{M-M}+ f_{y}^{M-F} \right) \dd a
       \dd y \big)}}{\splitfrac{\big( (1 - \sigma) \int_{y'=0}^\infty \int_{a'=y'}^\infty e^{-ra'} (1-\varsigma)d_{a'}^F \left(
   f_{y'}^{F-F} + f_{y'}^{F-M} \right) \dd a'\dd y'}{ +\sigma \int _{y=0}^\infty
   \int_{a=y}^\infty e^{-ra} \varsigma d_{a}^M \left( f_{y}^{M-M} + f_{y}^{M-F}
   \right) \dd a \dd y \big)}}
\end{equation}

Follow Equation~\eqref{eq:R0fromTy} to derive $R_0$ from $r$ and $T$. 

The stable sex ratio at birth, $S$ (and thencefrom $\varsigma$), is given from
the iterative calibration of $r$. From this, we can derive the stable
population sex ratio, $\bar{S}$:
\begin{equation}
\bar{S} = \frac{ \int_{y=0}^\infty \int_{a=y}^\infty e^{-ra} d_{a}^M \dd a \dd
y}{\int_{y'=0}^\infty \int_{a'=y'}^\infty e^{-ra'} d_{a'}^F \dd a' \dd
y'}
\end{equation}

The both-sex stable birth rate, $b$ is given by:
\begin{equation}
b = \frac{1}{
            \splitfrac{\big( \int _{y'=0}^\infty
            \int _{a'=y'}^\infty e^{-r a'} (1-\varsigma) d_{a'}^F \dd a' \dd
            y'}{ + \int _{y=0}^\infty \int _{a=y}^\infty
             e^{-r a} \varsigma d_{a}^M \dd a \dd y\big)}  }                   
\end{equation}
which can be used to derive the stable $e_y$-structure of males and females,
$c_y$ and $c_{y'}$, respectively:

\begin{equation}
c_{y'} = b (1-\varsigma) \int _{a'=y'}^\infty
e^{-ra'} d_{a'}^F \dd a'
\end{equation}
and
\begin{equation}
c_{y} = b \varsigma \int _{a=y}^\infty
e^{-ra} d_{a}^M \dd a'
\end{equation}
where:
\begin{equation}
1 = \int c_{y'} \dd y' + \int c_{y} \dd y
\end{equation}
