\documentclass{article}
\usepackage{amsmath}
\usepackage{natbib}
\bibpunct{(}{)}{,}{a}{}{;} 
\usepackage{url}
% for the d in integrals
\newcommand{\dd}{\; \mathrm{d}}
\begin{document}

\title{Dissertation errata: \\The two-sex problem in populations structured by
remaining years of life}
\author{Timothy L. M. Riffe}
\maketitle

Errors have been identified and amended in the following equations.
\begin{description}
\item[Equations 3.3 and 3.4]
\begin{align}
\intertext{Former:}
B^F &= \int_0^\infty m_a \dd a \notag \\
B^M &= \int_0^\infty m_{a'} \dd a'\notag \\
\intertext{Revised:}
B^F &= \int_0^\infty B^M(t-a)m_a \dd a \notag \\
B^M &= \int_0^\infty B^F(t-a)m_{a'} \dd a'\notag 
\end{align}
\item[Equation 3.9]
\begin{align}
\intertext{Former:}
1 &= \int _{a=0} ^\infty e^{-r a} \frac{F_a ^{M-M}}{v_0} p_a^m \dd a + \int
_{a'=0} ^\infty \frac{F_{a'} ^{F-F}}{1 - v_0} p_{a'}^f \dd a' \notag \\
\intertext{Revised:}
1 &= \int _{a=0} ^\infty e^{-r a} \frac{F_a ^{M-M}}{v_0} p_a^m \dd a + \int
_{a'=0} ^\infty e^{-r a'} \frac{F_{a'} ^{F-F}}{1 - v_0} p_{a'}^f \dd a' \notag
\end{align}
\item[Equation 3.43]
\begin{align}
\intertext{Former:}
c_a &=  \varsigma  e^{-ra} p_a^m \notag \\
\intertext{Revised:}
c_a &=  b\varsigma  e^{-ra} p_a^m \notag \\
\end{align}
\item[Equation 5.2] 
\begin{align}
\intertext{Former:}
B_t &= \int_{y=0}^\infty \int_{n=0}^\infty F_{y,t}
\frac{P_{n+y,t}d_{n+y,t}}{\int_{b=n+y}^\infty d_{b,t} \dd b} \dd y \notag\\
\intertext{Revised:}
B_t &= \int_{y=0}^\infty \int_{a=0}^\infty F_{y,t}
\frac{P_{a+y,t}d_{a+y,t}}{\int_{b=a+y}^\infty d_{b,t} \dd b} \dd a \dd y \notag
\end{align}
\item[Equation 5.3]
\begin{align}
\intertext{Former:}
B_t &= \int_{y=0}^\infty \int_{n=0}^\infty F_y
\frac{B_{t-n}d_{n+y}}{\int_{b=n+y}^\infty d_b \dd b} \dd n \dd y \notag\\
\intertext{Revised:}
B_t &= \int_{y=0}^\infty \int_{a=0}^\infty F_y B_{t-a}d_{a+y} \dd a \dd y \notag
\end{align}
\item[Equation 5.5]
\begin{align}
\intertext{Former:}
B_t &= \int_{y=0}^\infty \int_{a=0}^\infty F_y
\frac{B_{t}e^{-ra}d_{y+a}}{\int_{b=a+y}^\infty d_b \dd b} \dd a \dd y
\intertext{Revised:}
B_t &= \int_{y=0}^\infty \int_{a=0}^\infty F_y B_{t}e^{-ra}d_{a} \dd a \dd y
\end{align}


\item[Equation 5.6]
\begin{align}
\intertext{Former:}
B_t = \int_{y=0}^\infty \int_{n=0}^\infty F_y
\frac{B_{t}e^{-rn}d_{y+n}}{\int_{b=n+y}^\infty d_b \dd b} \dd n \dd y \notag\\
\intertext{Revised:}
B_t = \int_{y=0}^\infty \int_{a=0}^\infty F_y
\frac{B_{t}e^{-ra}d_{y+a}}{\int_{b=a+y}^\infty d_b \dd b} \dd a \dd y \notag
\end{align}
\item[Equation 5.9]
\begin{align}
\intertext{Former:}
1 &= \int _{a=0}^\infty \int _{b=a}^\infty e^{-ra} d_{b} m_a \dd b \dd a
\intertext{Revised:}
1 &= \int _{a=0}^\infty \int _{y = 0}^\infty e^{-ra} d_{a+y} m_a \dd y \dd a
\end{align}
\end{description}

\end{document}














